tweaks

examples/layeredeffects/parsing/FlightsStExn.fst
@@ -21,9 +21,7 @@ type state = {
 
 type pre_t = state -> HS.mem -> Type0
 type post_t (a:Type) = option (a & state) -> HS.mem -> Type0
-
-type wp_t0 (a:Type) =
-  wp:(post_t a -> pre_t)
+type wp_t0 (a:Type) = post_t a -> pre_t
 
 unfold
 let monotonic_wp (#a:Type) (wp:wp_t0 a) : Type0 =
@@ -31,17 +29,29 @@ let monotonic_wp (#a:Type) (wp:wp_t0 a) : Type0 =
     (forall r h. p r h ==> q r h) ==>
     (forall st h. wp p st h ==> wp q st h)
 
+type wp_t (a:Type) = wp:(post_t a -> pre_t){monotonic_wp wp}
 
-type wp_t (a:Type) =
-  wp:(post_t a -> pre_t){monotonic_wp wp}
-
-type repr (a:Type) (wp:wp_t a) =
+inline_for_extraction
+type mrepr (a:Type) (wp:wp_t a) =
   st:state -> EXN (a & state) (fun p h -> wp p st h)
 
 
+inline_for_extraction noextract
 let return (a:Type) (x:a)
-: repr a (fun p st h -> p (Some (x, st)) h)
+: mrepr a (fun p st h -> p (Some (x, st)) h)
 = fun st -> (x, st)
+
+open FStar.Tactics
+
+let lemma_monotonic
+  (#a:Type) (#b:Type)
+  (wp_f:wp_t a) (wp_g:a -> wp_t b)
+  (post_a:(a:Type -> b:Type -> wp_g:(a -> wp_t b) -> p:post_t b -> post_t a))
+  (p:post_t b) (q:post_t b) (st:state) (h:HS.mem)
+: Lemma
+  (requires forall (r:option (a & state)) (h:HS.mem). (post_a a b wp_g p) r h ==> (post_a a b wp_g q) r h)
+  (ensures wp_f (post_a a b wp_g p) st h ==> wp_f (post_a a b wp_g q) st h)
+= ()
 
 unfold
 let post_a (a:Type) (b:Type) (wp_g:a -> wp_t b) (p:post_t b) : post_t a =
@@ -50,50 +60,77 @@ let post_a (a:Type) (b:Type) (wp_g:a -> wp_t b) (p:post_t b) : post_t a =
   | None -> p None h
   | Some r -> Prims.auto_squash (wp_g (Mktuple2?._1 r) p (Mktuple2?._2 r) h)
 
-let lemma_monotonic2 (#a:Type) (#b:Type) (wp_f:wp_t a) (wp_g:a -> wp_t b) (p:post_t b) (q:post_t b) (st:state) (h:HS.mem)
-: Lemma
-  (requires forall (r:option (a & state)) (h:HS.mem). (post_a a b wp_g p) r h ==> (post_a a b wp_g q) r h)
-  (ensures wp_f (post_a a b wp_g p) st h ==> wp_f (post_a a b wp_g q) st h)
-= let aux (p q:post_t a)
-    : Lemma ((forall r h. p r h ==> q r h) ==> (forall st h. wp_f p st h ==> wp_f q st h))
-    = () in
-  aux (post_a a b wp_g p) (post_a a b wp_g q);
-  admit ()
+unfold
+let bind_wp0 (#a:Type) (#b:Type) (wp_f:wp_t a) (wp_g:a -> wp_t b) : wp_t0 b =
+  fun p -> wp_f (post_a a b wp_g p)
 
 unfold
-let bind_wp0 (a:Type) (b:Type) (wp_f:wp_t a) (wp_g:a -> wp_t b) : post_t b -> pre_t =
-  fun p st h -> wp_f (post_a a b wp_g p) st h
-
-open FStar.Tactics
-
-unfold
-let bind_wp (a:Type) (b:Type) (wp_f:wp_t a) (wp_g:a -> wp_t b) : wp_t b
-= assert (monotonic_wp (bind_wp0 a b wp_f wp_g)) by
-    (norm [delta_only [`%monotonic_wp]];
-     let p_binder = forall_intro () in
-     let q_binder = forall_intro () in
-     ignore (implies_intro ());
-     ignore (forall_intro ());
-     norm [delta_only [`%bind_wp0]];
-     ignore (forall_intro ());
-     let wp_f_binder, wp_g_binder =
+let bind_wp (#a:Type) (#b:Type) (wp_f:wp_t a) (wp_g:a -> wp_t b) : wp_t b
+= assert (monotonic_wp (bind_wp0 wp_f wp_g)) by
+    (norm [delta_only [`%monotonic_wp; `%bind_wp0]];
+     (ignore (repeatn 5 l_intro));
+     let wp_f, wp_g =
        match (cur_binders ()) with
        | _::_::wp_f::wp_g::_ -> wp_f, wp_g
        | _ -> fail "" in
-     apply_lemma (`(lemma_monotonic2 (`#(binder_to_term wp_f_binder)) (`#(binder_to_term wp_g_binder)) (`#(binder_to_term p_binder)) (`#(binder_to_term q_binder))));
-     norm [delta_only [`%post_a]];
-     ignore (forall_intro ()));
-  bind_wp0 a b wp_f wp_g
+     apply_lemma (`(lemma_monotonic
+       (`#(binder_to_term wp_f))
+       (`#(binder_to_term wp_g))
+       post_a));
+     norm [delta_only [`%post_a]]);
+  bind_wp0 wp_f wp_g
 
-inline_for_extraction
+inline_for_extraction noextract
 let bind (a:Type) (b:Type)
   (wp_f:wp_t a) (wp_g:a -> wp_t b)
-  (f:repr a wp_f) (g:(x:a -> repr b (wp_g x)))
-: repr b (bind_wp a b wp_f wp_g)
+  (f:mrepr a wp_f) (g:(x:a -> mrepr b (wp_g x)))
+: mrepr b (bind_wp wp_f wp_g)
 = fun st ->
   let (x, st) = f st in
   g x st
 
+inline_for_extraction noextract
+let stronger (a:Type)
+  (wp_f:wp_t a) (wp_g:wp_t a)
+  (f:mrepr a wp_f)
+: Pure (mrepr a wp_g)
+  (requires forall p st h. wp_g p st h ==> wp_f p st h)
+  (ensures fun _ -> True)
+= f
+
+inline_for_extraction noextract
+let conjunction (a:Type)
+  (wp_f:wp_t a) (wp_g:wp_t a)
+  (f:mrepr a wp_f) (g:mrepr a wp_g)
+  (p:Type0)
+: Type
+= mrepr a
+  (fun post st h ->
+    (p ==> wp_f post st h) /\
+    (( ~p) ==> wp_g post st h))
+
+
+reifiable reflectable
+layered_effect {
+  STEXN : a:Type -> wp_t a -> Effect
+  with
+  repr = mrepr;
+  return = return;
+  bind = bind;
+  stronger = stronger;
+  conjunction = conjunction
+}
+
+inline_for_extraction noextract
+let lift_div_stexn (a:Type) (wp:pure_wp a{forall p q. (forall x. p x ==> q x) ==> (wp p ==> wp q)}) (f:unit -> DIV a wp)
+: mrepr a (fun p st h -> wp (fun x -> p (Some (x, st)) h))
+= fun st -> (f (), st)
+
+sub_effect DIV ~> STEXN = lift_div_stexn
+
+
+effect StExn (a:Type) (pre:state -> HS.mem -> Type0) (post:state -> HS.mem -> option (a & state) -> HS.mem -> Type) =
+  STEXN a (fun p st h -> pre st h /\ (forall r h1. (equal_stack_domains h h1 /\ post st h r h1) ==> p r h1))
 
 type repr (a:Type0) = {
   v       : a;
@@ -104,6 +141,44 @@ type repr (a:Type0) = {
 let valid_repr (#a:Type0) (b:B.buffer uint_8) (h:HS.mem) (r:repr a) : Type0
 = valid_parsing b r.m_begin r.m_end h r.v
 
+unfold let pre_m (st:state) (h:HS.mem) = B.live h st.b
+
+unfold let post_m (#a:Type0) (st:state) (h0:HS.mem) (r:option (repr a & state)) (h1:HS.mem) =
+  B.(modifies loc_none h0 h1) /\
+  (match r with
+   | None -> True
+   | Some (x, st1) ->
+     st1.b == st.b /\
+     x.m_begin == st.id /\
+     x.m_end == st1.id /\
+     valid_repr #a st1.b h1 x)
+
+inline_for_extraction noextract
+let parse_common_ (#a:Type0)
+  (parser:parser_t a)
+  (_:unit)
+  (st:state)
+  (_:unit)
+: ST (option (repr a & state)) (requires pre_m st) (ensures post_m st)
+= let r = parser st.b st.id in
+  match r with
+  | None -> None
+  | Some (x, m_end) -> Some ({ v = x; m_begin = st.id; m_end = m_end }, { st with id = m_end })
+
+inline_for_extraction noextract
+let parse_common_exn (#a:Type0)
+  (parser:parser_t a)
+  (_:unit)
+  (st:state)
+: Exn (repr a & state) (requires pre_m st) (ensures post_m st)
+= EXN?.reflect (parse_common_ #a parser () st)
+
+inline_for_extraction noextract
+let parse_common (#a:Type0)
+  (parser:parser_t a)
+  (_:unit)
+: StExn (repr a) (requires pre_m) (ensures post_m)
+= STEXN?.reflect (parse_common_exn #a parser ())
 
 noeq
 type flt = {
@@ -113,62 +188,36 @@ type flt = {
 }
 
 
-unfold let pre_m (b:B.buffer uint_8) m_begin =
-  fun h -> B.live h b /\ m_begin <= B.len b
-
-unfold let post_m (#a:Type0) b =
-  fun h0 r h1 ->
-  B.(modifies loc_none h0 h1) /\
-  (match r with
-   | None -> True
-   | Some x -> valid_repr b h1 x)
-
-inline_for_extraction
-let parse_common_ (#a:Type0)
-  (parser:parser_t a)
-  (b:B.buffer uint_8)
-  (m_begin:uint_32)
-: unit -> ST (option (repr a)) (requires pre_m b m_begin) (ensures post_m #a b)
-= fun _ ->
-  let r = parser b m_begin in
-  match r with
-  | None -> None
-  | Some (x, m_end) -> Some ({ v = x; m_begin = m_begin; m_end = m_end })
-
-inline_for_extraction
-let parse_common (#a:Type0) (parser:parser_t a) (b:B.buffer uint_8) (m_begin:uint_32)
-: Exn (repr a) (requires pre_m b m_begin) (ensures post_m #a b)
-= EXN?.reflect (parse_common_ #a parser b m_begin)
-
-inline_for_extraction
+inline_for_extraction noextract
 let parse_t1 = parse_common #t1 t1_parser
 
-inline_for_extraction
+inline_for_extraction noextract
 let parse_t2 = parse_common #t2 t2_parser
 
-inline_for_extraction
+inline_for_extraction noextract
 let parse_t3 = parse_common #t3 t3_parser
 
-unfold let pre_f (b:B.buffer uint_8) f_begin f_end =
-  fun h -> B.live h b /\ valid_indices b f_begin f_end
-
-unfold let post_f (b:B.buffer uint_8) =
-  fun h0 r h1 ->
-   B.(modifies loc_none h0 h1) /\
-   (match r with
-    | None -> True
-    | Some flt -> valid_repr b h1 flt.t1_msg /\ valid_repr b h1 flt.t2_msg /\ valid_repr b h1 flt.t3_msg)
-
-inline_for_extraction
-let parse_flt_aux (b:B.buffer uint_8) (f_begin:uint_32) (f_end:uint_32)
-: Exn flt (requires pre_f b f_begin f_end) (ensures post_f b)
-= let x = parse_t1 b f_begin in
-  let y = parse_t2 b x.m_end in
-  let z = parse_t3 b y.m_end in
-  { t1_msg = x;
-    t2_msg = y;
-    t3_msg = z }
+inline_for_extraction noextract
+let parse_flt_aux ()
+: StExn flt
+  (fun st h -> B.live h st.b)
+  (fun st h0 r h1 ->
+    B.(modifies loc_none h0 h1) /\
+    (match r with
+     | None -> True
+     | Some (flt, _) ->
+       valid_repr st.b h1 flt.t1_msg /\ valid_repr st.b h1 flt.t2_msg /\ valid_repr st.b h1 flt.t3_msg))
+= let x = parse_t1 () in
+  let y = parse_t2 () in
+  let z = parse_t3 () in
+  { t1_msg = x; t2_msg = y; t3_msg = z }
 
 let parse_flt (b:B.buffer uint_8) (f_begin:uint_32) (f_end:uint_32)
-: ST (option flt) (requires pre_f b f_begin f_end) (ensures post_f b)
-= reify (parse_flt_aux b f_begin f_end) ()
+: ST (option (flt & state))
+  (requires fun h -> B.live h b /\ valid_indices b f_begin f_end)
+  (ensures fun h0 r h1 ->
+    B.(modifies loc_none h0 h1) /\
+    (match r with
+     | None -> True
+     | Some (flt, _) -> valid_repr b h1 flt.t1_msg /\ valid_repr b h1 flt.t2_msg /\ valid_repr b h1 flt.t3_msg))
+= reify (reify (parse_flt_aux ()) ({ b = b; id = f_begin })) ()
